scall spec done, started refactoring LSE example to work on arbitrary program adresses, using the scall spec

theories/examples/lse.v
@@ -43,6 +43,11 @@ Section lse.
            apply incr_list_le_middle with a index; auto ]
     end.
 
+  Ltac isWithinBounds := rewrite /withinBounds; apply andb_true_iff; split; apply Z.leb_le; simpl; auto.
+
+  Ltac iNotElemOfList :=
+    repeat (apply not_elem_of_cons; split;[auto|]); apply not_elem_of_nil.  
+
   Ltac addr_succ :=
     match goal with
     | H : _ |- (?a1 + ?z)%a = Some ?a2 =>
@@ -82,332 +87,181 @@ Section lse.
    Ltac get_genpur_reg Hr_gen wsr ptr :=
      let w := fresh "wr" in 
        destruct wsr as [? | w wsr]; first (by iApply bi.False_elim);
-       iDestruct Hr_gen as ptr. 
+       iDestruct Hr_gen as ptr.
+
+   Ltac iDestructList Hlength l :=
+     (repeat (let a := fresh "a" in destruct l as [|a l];[by inversion Hlength|]));
+     destruct l;[|by inversion l].
+   
+   Ltac iContiguous_bounds lo mid hi index Ha :=
+     split; [apply incr_list_ge_middle with _ index lo mid in Ha; auto|
+             apply incr_list_le_middle with _ index mid hi in Ha; auto]. 
+
+   Ltac iContiguous_next Ha index :=
+     rewrite /contiguous in Ha; apply Ha with index;auto.
     
         
   (* encapsulation of local state using local capabilities and scall *)
   (* assume r1 contains an executable pointer to adversarial code 
      (no linking table yet) *)
-  Definition f2 (r1 : RegName) (p : Perm) : iProp Σ :=
-    (    (* push 1 *)
-           push_z (a-0) (a-1) p r_stk 1
-    (* (* scall r1([],[]) *) *)
-    (*      (* push private state *) *)
-    (*      (* push activation code *) *)
-    (*      ∗ push_z (a-2) (a-3) p r_stk w_1 *)
-    (*      ∗ push_z (a-4) (a-5) p r_stk w_2 *)
-    (*      ∗ push_z (a-6) (a-7) p r_stk w_3 *)
-    (*      ∗ push_z (a-8) (a-9) p r_stk w_4a *)
-    (*      ∗ push_z (a-10) (a-11) p r_stk w_4b *)
-    (*      ∗ push_z (a-12) (a-13) p r_stk w_4c *)
-    (*      (* push old pc *) *)
-    (*      ∗ (a-14) ↦ₐ[p] move_r r_t1 PC *)
-    (*      ∗ (a-15) ↦ₐ[p] lea_z r_t1 64 (* offset to "after" *) *)
-    (*      ∗ push_r (a-16) (a-17) p r_stk r_t1 *)
-    (*      (* push stack pointer *) *)
-    (*      ∗ (a-18) ↦ₐ[p] lea_z r_stk 1 *)
-    (*      ∗ (a-19) ↦ₐ[p] store_r r_stk r_stk *)
-    (*      (* set up protected return pointer *) *)
-    (*      ∗ (a-20) ↦ₐ[p] move_r r_t0 r_stk *)
-    (*      ∗ (a-21) ↦ₐ[p] lea_z r_t0 (-7)%Z *)
-    (*      ∗ (a-22) ↦ₐ[p] restrict_z r_t0 (local_e) *)
-    (*      (* restrict stack capability *) *)
-    (*      ∗ (a-23) ↦ₐ[p] geta r_t1 r_stk *)
-    (*      ∗ (a-24) ↦ₐ[p] add_r_z r_t1 r_t1 1 *)
-    (*      ∗ (a-25) ↦ₐ[p] gete r_t2 r_stk *)
-    (*      ∗ (a-26) ↦ₐ[p] subseg_r_r r_stk r_t1 r_t2 *)
-    (*      (* clear the unused part of the stack *) *)
-    (*      (* mclear r_stk: *) *)
-    (*      ∗ mclear (region_addrs_aux (a-27) 22) p r_stk 10 2 (* contiguous *) *)
-    (*      (* clear non-argument registers *) *)
-    (*      ∗ rclear (region_addrs_aux (a-49) 29) p *)
-    (*               (list_difference all_registers [PC;r_stk;r_t0;r1]) *)
-    (*      (* jump to unknown code *) *)
-    (*      ∗ (a-78) ↦ₐ[p] jmp r1 *)
-         ∗ scall_prologue (region_addrs (a-2) (a-77)) p 64 r1
-         (* jump to unknown code *)
-         ∗ (a-78) ↦ₐ[p] jmp r1
-    (* after: *)
-         (* pop the restore code *)
-         (* to shorten the program we will do it all at once *)
-         ∗ (a-79) ↦ₐ[p] sub_z_z r_t1 0 7
-         ∗ (a-80) ↦ₐ[p] lea_r r_stk r_t1
-         (* pop the private state into appropriate registers *)
-    (* END OF SCALL *)
-         ∗ (a-81) ↦ₐ[p] load_r r1 r_stk
-         ∗ (a-82) ↦ₐ[p] sub_z_z r_t1 0 1
-         ∗ (a-83) ↦ₐ[p] lea_r r_stk r_t1
-         (* assert r1 points to 1. For "simplicity" I am not using the assert macro ! 
-            but rather a hardcoded version for f2. TODO: change this to actual assert *)
-         ∗ (a-84) ↦ₐ[p] move_r r_t1 PC
-         ∗ (a-85) ↦ₐ[p] lea_z r_t1 5(* offset to fail *)
-         ∗ (a-86) ↦ₐ[p] sub_r_z r1 r1 1
-         ∗ (a-87) ↦ₐ[p] jnz r_t1 r1
-         ∗ (a-88) ↦ₐ[p] halt
-         (* set the flag to 1 to indicate failure. flag is set to be the address after 
-            the program *)
-         ∗ (a-89) ↦ₐ[p] move_r r_t1 PC
-         ∗ (a-90) ↦ₐ[p] lea_z r_t1 4(* offset to flag *)
-         ∗ (a-91) ↦ₐ[p] store_z r_t1 1
-         ∗ (a-92) ↦ₐ[p] halt
-    )%I.
+   Definition f2_instrs (r1 : RegName) epilogue_off flag_off :=
+     push_z_instrs r_stk 1 ++
+     scall_prologue_instrs epilogue_off r1 ++
+     [jmp r1;
+     sub_z_z r_t1 0 7;
+     lea_r r_stk r_t1;
+     load_r r1 r_stk;
+     sub_z_z r_t1 0 1;
+     lea_r r_stk r_t1;
+     move_r r_t1 PC;
+     lea_z r_t1 5; (* offset to assertion failure *)
+     sub_r_z r1 r1 1;
+     jnz r_t1 r1;
+     halt;
+     (* failure *)
+     move_r r_t1 PC;
+     lea_z r_t1 flag_off;
+     store_z r_t1 1;
+     halt].
 
+  Definition f2 (a : list Addr) (p : Perm) (r1 : RegName) epilogue_off flag_off : iProp Σ :=
+    ([∗ list] a_i;w_i ∈ a;(f2_instrs r1 epilogue_off flag_off), a_i ↦ₐ[p] w_i)%I.
+
+  Compute (length (f2_instrs (r_t30) 0 0)).
+  Compute (region_size (a-0) (a-93)).
 
   (* We want to show encapsulation of local state, by showing that an arbitrary adv 
      cannot change what lies on top of the stack after return, i.e. we want to show
      that the last pop indeed loads the value 1 into register r1 *)
   (* to make the proof simpler, we are assuming WLOG the r1 registers is r_t30 *)
-  Lemma f2_spec W b e a pc_p pc_g pc_b pc_e :
-    (* r1 ≠ PC ∧ r1 ≠ r_stk ∧ r1 ≠ r_t0 → *)
-    isCorrectPC (inr ((pc_p,pc_g),pc_b,pc_e,(a-0))) ∧
-    isCorrectPC (inr ((pc_p,pc_g),pc_b,pc_e,(a-110))) →
-    {{{ r_stk ↦ᵣ inr ((RWLX,Local),(a-120),(a-150),(a-119))
+  Lemma f2_spec W b e a pc_p pc_g pc_b pc_e (* PC *)
+        f2_addrs flag_off (* f2 *)
+        a_first a_last a_flag (* special adresses *) 
+        (b_r e_r b_r' : Addr) (* stack *) :
+    
+    (* PC assumptions *)
+    isCorrectPC (inr ((pc_p,pc_g),pc_b,pc_e,a_first)) ∧
+    isCorrectPC (inr ((pc_p,pc_g),pc_b,pc_e,a_last)) →
+
+    (* Program adresses assumptions *)
+    contiguous f2_addrs ->
+    f2_addrs !! 0 = Some a_first ∧ list.last f2_addrs = Some a_last ->
+    
+    (* Stack assumptions *)
+    (0%a ≤ e_r)%Z ∧ (0%a ≤ b_r)%Z -> (* this assumption will not be necessary once addresses are finite *)
+    (b_r ≤ e_r)%Z ->
+    region_size b_r e_r > 10 -> (* we must assume the stack is large enough for needed local state *)
+    (b_r' + 1)%a = Some b_r ->
+    
+    {{{ r_stk ↦ᵣ inr ((RWLX,Local),b_r,e_r,b_r')
       ∗ (∃ wsr, [∗ list] r_i;w_i ∈ list_difference all_registers [PC;r_stk;r_t30]; wsr,
            r_i ↦ᵣ w_i)
-      ∗ (∃ ws, [[(a-120), (a-150)]]↦ₐ[RWLX][[ws]])
+      ∗ (∃ ws, [[b_r, e_r]]↦ₐ[RWLX][[ws]])
       (* flag *)
-      ∗ (a-93) ↦ₐ[RW] inl 0%Z
+      ∗ a_flag ↦ₐ[RW] inl 0%Z
       (* token which states all invariants are closed *)
       ∗ na_own logrel_nais ⊤
       (* adv *)
       ∗ r_t30 ↦ᵣ inr ((E,Global),b,e,a)
       ∗ ([∗ list] a ∈ region_addrs b e, read_write_cond a RX interp)
       (* trusted *)
-      ∗ PC ↦ᵣ inr ((pc_p,pc_g),pc_b,pc_e,(a-0))
-      ∗ f2 r_t30 pc_p
+      ∗ PC ↦ᵣ inr ((pc_p,pc_g),pc_b,pc_e,a_first)
+      ∗ f2 f2_addrs pc_p r_t30 65 flag_off
       (* we start out with arbitrary sts *)
       ∗ sts_full_world sts_std W
       ∗ region W
     }}}
       Seq (Instr Executable)
-    {{{ v, RET v; ⌜v = HaltedV⌝ → (a-93) ↦ₐ[RW] inl 0%Z }}}.
+    {{{ v, RET v; ⌜v = HaltedV⌝ → a_flag ↦ₐ[RW] inl 0%Z }}}.
   Proof.
-    iIntros ([Hvpc0 Hvpc93] φ)
-        "(Hr_stk & Hr_gen & Hstack & Hflag & Hna & Hr1 & #Hadv & HPC & Hf2 & Hs & Hr) Hφ /=".
+    iIntros ([Hvpc0 Hvpc93] Hf2 [Ha_first Ha_last] Hbounds Hle Hsize Hb_r' φ)
+            "(Hr_stk & Hr_gen & Hstack & Hflag & Hna & Hr1 & #Hadv & HPC & Hf2 & Hs & Hr) Hφ /=".
+    (* Getting some general purpose regiters *)
     iDestruct "Hr_gen" as (wsr) "Hr_gen". 
-    get_genpur_reg "Hr_gen" wsr "[Hrt0 Hr_gen]".
-    get_genpur_reg "Hr_gen" wsr "[Hrt1 Hr_gen]".
-    get_genpur_reg "Hr_gen" wsr "[Hrt2 Hr_gen]". 
+    (* get_genpur_reg "Hr_gen" wsr "[Hrt0 Hr_gen]". *)
+    (* get_genpur_reg "Hr_gen" wsr "[Hrt1 Hr_gen]". *)
+    (* get_genpur_reg "Hr_gen" wsr "[Hrt2 Hr_gen]". *)
+    (* assert that the stack bounds are within bounds *)
+    assert (withinBounds (RWLX,Local,b_r,e_r,b_r) = true ∧ withinBounds (RWLX,Local,b_r,e_r,e_r) = true) as [Hwb1 Hwb2].
+    { split; isWithinBounds; lia. }
+    (* Splitting the stack into own and adv parts *)
     iDestruct "Hstack" as (ws) "Hstack". 
     iDestruct (big_sepL2_length with "Hstack") as %Hlength.
     assert (∃ ws_own ws_adv, ws = ws_own ++ ws_adv ∧ length ws_own = 9)
       as [ws_own [ws_adv [Happ Hlength'] ] ].
-    { simpl in Hlength.
-      do 9 (destruct ws as [|? ws]; inversion Hlength).
-        by exists [w;w0;w1;w2;w3;w4;w5;w6;w7],ws. }
-    assert ((a-100 ≤ a-108)%Z ∧ (a-108 < a-150)%Z); first (simpl; lia).  
-    rewrite Happ (stack_split (a-120) (a-150) (a-128) (a-129)); auto; try addr_succ.
-    simpl in Hlength. 
-    iDestruct "Hstack" as "[Hstack_own Hstack_adv]".
-    rewrite /region_mapsto.
-    assert (region_addrs (a-120) (a-128) = [a-120;a-121;a-122;a-123;a-124;a-125;a-126;a-127;a-128])
-      as ->.
-    { rewrite /region_addrs. 
-      simpl. repeat f_equal; (apply eq_proofs_unicity; decide equality). }
-    wp_push_z "Hstack_own" (a-0) (a-110) (a-120) (a-150) (a-119) (a-120) φ (a-0) (a-1) (a-2) ws_own "Hf2"
-              "(HPC & _ & Hr_stk & Ha120)".
-    iDestruct "Hf2" as "[Hscall Hf2]". 
-    iApply (scall_prologue_spec (a-128) (a-129) (a-121) (a-79) (a-78) with "[-]");
-      last iFrame "HPC Hr_stk Hscall";
-      try addr_succ;[apply isCorrectPC_bounds with (a-0) (a-110); auto|apply isCorrectPC_bounds with (a-0) (a-110); auto|apply PermFlows_refl|..]. 
-    iSplitL "Hr_gen Hrt0 Hrt1 Hrt2"; [admit|].
-    iSplitL "Hstack";[admit|].
-    iSplitL "Hstack_adv";[admit|]. 
+    { rewrite region_addrs_length in Hlength; auto. rewrite Hlength in Hsize. 
+      do 9 (destruct ws as [|? ws]; [simpl in Hsize; lia|]).
+           by exists [w;w0;w1;w2;w3;w4;w5;w6;w7],ws. }
+    rewrite Happ.
+    iDestruct (contiguous_program_split with "Hstack") as (stack_own stack_adv s_last s_first)
+                                                            "(Hstack_own & Hstack_adv & #Hcont)";
+      [apply region_addrs_contiguous|lia|..].
+    { rewrite Happ region_addrs_length in Hlength;[|auto]. rewrite app_length in Hlength. lia. }
+    iDestruct "Hcont" as %(Hstack_own & Hstack_adv & Hstackeq & Hs_last & Hs_first & Hlink).
+    assert (contiguous (region_addrs b_r e_r)) as Hstackcont;[apply region_addrs_contiguous|rewrite Hstackeq in Hstackcont]. 
+    iDestruct (big_sepL2_length with "Hstack_own") as %Hlength_own. rewrite Hlength' in Hlength_own.
+    (* Getting the top adress on the stack *)
+    destruct stack_own as [|a0 stack_own]; [inversion Hlength_own|]; destruct ws_own as [|w ws_own];[inversion Hlength'|].
+    iDestruct "Hstack_own" as "[Ha0 Hstack_own]".
+    (* Prepare the push macro *)
+    rewrite /f2 /f2_instrs. 
+    iDestruct (contiguous_program_split with "Hf2") as (push_z rest push_z_last rest_first)
+                                                         "(Hpush & Hf2 & #Hcont)"; [auto|simpl;lia|simpl;lia|..]. 
+    iDestruct "Hcont" as %(Hpush & Hrest & Hprogeq & Hp_last & Hp_first & Hlink').
+    iDestruct (big_sepL2_length with "Hpush") as %Hpush_length.
+    iDestructList Hpush_length push_z.
+    assert (a1 = a_first) as ->;[subst; by inversion Ha_first|simplify_eq].
+    assert (a0 = b_r) as ->;[|simplify_eq].
+    { assert ((region_addrs b_r e_r) !! 0 = Some b_r) as Hfirst;[apply region_addrs_first;auto|].
+      rewrite Hstackeq in Hfirst. by inversion Hfirst. }
+    assert (a2 = push_z_last) as <-;[|simplify_eq];[simpl in Hp_last; by inversion Hp_last|].
+    (* push 1 *)
+    iApply (push_z_spec with "[-]"); last iFrame "Hpush HPC Ha0 Hr_stk";
+      [|apply PermFlows_refl|isWithinBounds;lia|iContiguous_next Hf2 0|apply Hlink'|apply Hb_r'|..].
+    { split; auto. apply isCorrectPC_bounds_alt with a_first a_last; auto. iContiguous_bounds a_first a2 a_last 1 Hf2. }
+    iNext. iIntros "(HPC & _ & Hr_stk & Hb_r)".
+    (* Prepare the scall prologue macro *)
+    destruct stack_own as [|stack_own_b stack_own];[inversion Hlength_own|]. 
+    assert ((stack_own_b :: stack_own) = region_addrs stack_own_b s_last) as ->.
+    { apply contiguous_region_addrs; auto. by apply contiguous_weak in Hstack_own. }
+    assert (stack_adv = region_addrs s_first e_r) as ->.
+    { apply contiguous_region_addrs; auto. rewrite -(region_addrs_last b_r);[|auto].
+      rewrite Hstackeq. rewrite -last_app_eq; [auto|]. destruct stack_adv; [inversion Hs_first|simpl;lia]. }
+    iDestruct (contiguous_program_split with "Hf2") as (scall_prologue rest0 scall_last rest0_first)
+                                                         "(Hscall & Hf2 & #Hcont)"; [auto|simpl;lia|simpl;lia|..].
+    clear Hlink' Hp_last.
+    iDestruct "Hcont" as %(Hcont_scall & Hcont_rest0 & Hrest_app & Hscall_last & Hrest0_first & Hlink'). subst.
+    iDestruct (big_sepL2_length with "Hscall") as %Hscall_length. simpl in Hscall_length.
+    assert ((stack_own_b + 7)%a = Some s_last) as Hstack_own_bound.
+    { apply (contiguous_incr_addr_middle _ 1 7 stack_own_b _ Hstack_own); auto. simpl.
+      assert (length stack_own - 1 = 6) as Heq;[simpl in Hlength_own;lia|]. rewrite -Heq. 
+      rewrite -last_lookup. simpl in Hs_last. destruct stack_own; [inversion Heq|done]. }
+    (* scall *)
+    iApply (scall_prologue_spec with "[-]");
+      last ((iFrame "HPC Hr_stk Hscall"); iSplitL "Hr_gen";[iNext;simpl;iExists wsr;iFrame|
+                                          iSplitL "Hstack_own";[iNext;iExists ws_own;iFrame|
+                                                                iSplitL "Hstack_adv";[iNext;iExists ws_adv;iFrame|] ] ]);
+      [| | | |apply Hbounds|apply Hcont_scall|rewrite -(lookup_app_l _ rest0);[auto|rewrite Hscall_length;simpl;lia] |apply Hscall_last|
+       apply PermFlows_refl|iNotElemOfList|iContiguous_next Hstack_own 0|apply Hstack_own_bound| | |apply Hlink'|..].
+    { apply isCorrectPC_bounds_alt with a_first a_last; auto. iContiguous_bounds a_first rest_first a_last 2 Hf2. }
+    { apply isCorrectPC_bounds_alt with a_first a_last; auto. iContiguous_bounds a_first scall_last a_last 78 Hf2;
+      (rewrite lookup_app_r;[|simpl;lia]; rewrite lookup_app_l;[simpl|rewrite Hscall_length;simpl;lia];
+      assert (length scall_prologue - 1 = 76) as <-;[subst;lia|]; by rewrite -last_lookup). }
+    { apply isWithinBounds_bounds_alt with b_r e_r; auto. iContiguous_bounds b_r stack_own_b e_r 1 Hstackcont.
+      apply last_app_region_addrs. destruct (region_addrs s_first e_r); [inversion Hs_first|simpl;lia]. }
+    { apply isWithinBounds_bounds_alt with b_r e_r; auto. iContiguous_bounds b_r s_first e_r (2 + length stack_own) Hstackcont;
+      [rewrite lookup_app_r /=; auto; by rewrite PeanoNat.Nat.sub_diag..|].
+      apply last_app_region_addrs. destruct (region_addrs s_first e_r); [inversion Hs_first|simpl;lia]. }
+    { assert (8 = 7 + 1)%Z as ->;[lia|]. rewrite (addr_add_assoc _ s_last); auto. }
+    { apply (contiguous_incr_addr _ 77 rest_first _ Hrest); auto.
+      rewrite lookup_app_r;[|lia]. by rewrite -Hscall_length PeanoNat.Nat.sub_diag. }
     iNext. iIntros "(HPC & Hr_stk & Hr_t0 & Hr_gen & Hstack_own & Hstack_adv & _)". 
-    
-
-
-
-
-    
-
-    (*
-    wp_push_z "Hstack" (a-0) (a-110) (a-120) (a-150) (a-120) (a-121) φ (a-2) (a-3) (a-4) ws_own "Hf2"
-              "(HPC & _ & Hr_stk & Ha121)".
-    wp_push_z "Hstack" (a-0) (a-110) (a-120) (a-150) (a-121) (a-122) φ (a-4) (a-5) (a-6) ws_own "Hf2"
-              "(HPC & _ & Hr_stk & Ha122)".
-    wp_push_z "Hstack" (a-0) (a-110) (a-120) (a-150) (a-122) (a-123) φ (a-6) (a-7) (a-8) ws_own "Hf2"
-              "(HPC & _ & Hr_stk & Ha123)".
-    wp_push_z "Hstack" (a-0) (a-110) (a-120) (a-150) (a-123) (a-124) φ (a-8) (a-9) (a-10) ws_own "Hf2"
-              "(HPC & _ & Hr_stk & Ha124)".
-    wp_push_z "Hstack" (a-0) (a-110) (a-120) (a-150) (a-124) (a-125) φ (a-10) (a-11) (a-12) ws_own "Hf2"
-              "(HPC & _ & Hr_stk & Ha125)".
-    wp_push_z "Hstack" (a-0) (a-110) (a-120) (a-150) (a-125) (a-126) φ (a-12) (a-13) (a-14) ws_own "Hf2"
-              "(HPC & _ & Hr_stk & Ha126)".
-    iDestruct "Hf2" as "[Hi Hf2]".
-    iApply (wp_bind (fill [SeqCtx])).
-    iApply (wp_move_success_reg_fromPC _ _ _ _ _ (a-14) (a-15) _ r_t1
-              with "[Hi Hrt1 HPC]"); eauto; try addr_succ;
-      first apply move_r_i; first apply PermFlows_refl;
-      first (apply isCorrectPC_bounds with (a-0) (a-110); eauto; split; done).
-    iFrame. iNext. iIntros "(HPC & _ & Hr_t1)". iSimpl.
-    iDestruct "Hf2" as "[Hi Hf2]".
-    iApply wp_pure_step_later;auto;iNext. 
-    iApply (wp_bind (fill [SeqCtx])).
-    iApply (wp_lea_success_z _ _ _ _ _ (a-15) (a-16) _ r_t1 pc_p _ _ _ (a-14) 64 (a-78)
-              with "[Hi Hr_t1 HPC]"); eauto; try addr_succ;
-      first apply lea_z_i; first apply PermFlows_refl;
-      first (apply isCorrectPC_bounds with (a-0) (a-110); eauto; split; done).
-    { inversion Hvpc0 as [?????? Hpc_p]; 
-        destruct Hpc_p as [Hpc_p | [Hpc_p | Hpc_p] ]; congruence. }
-    iFrame. iNext. iIntros "(HPC & _ & Hrt_1)"; iSimpl.
-    iApply wp_pure_step_later;auto;iNext. 
-    wp_push_r "Hstack" (a-0) (a-110) (a-120) (a-150) (a-126) (a-127) φ (a-16) (a-17) (a-18) ws_own "Hf2"
-              "(HPC & _ & Hr_stk & Hr_t1 & Ha127)".
-    iDestruct "Hf2" as "[Hi Hf2]".
-    iApply (wp_bind (fill [SeqCtx])).
-    iApply (wp_lea_success_z _ _ _ _ _ (a-18) (a-19) _ r_stk RWLX _ _ _ (a-127) 1 (a-128)
-              with "[Hi Hr_stk HPC]"); eauto; try addr_succ;
-      first apply lea_z_i; first apply PermFlows_refl;
-      first (apply isCorrectPC_bounds with (a-0) (a-110); eauto; split; done).
-    iFrame. iNext. iIntros "(HPC & _ & Hr_stk)"; iSimpl.
-    iApply wp_pure_step_later;auto;iNext.
-    destruct ws_own as [_ | wa129 ws_own]; first inversion Hlength';
-      iDestruct "Hstack" as "[Ha128 Hstack]".
-    iDestruct "Hf2" as "[Hi Hf2]".
-    iApply (wp_bind (fill [SeqCtx])).
-    iApply (wp_store_success_reg_same _ _ _ _ _ (a-19) (a-20) _ r_stk _ RWLX
-                                 Local (a-120) (a-150) (a-128)
-              with "[HPC Hi Hr_stk Ha128]"); eauto; try addr_succ;
-      first apply store_r_i; try apply PermFlows_refl;
-      first (apply isCorrectPC_bounds with (a-0) (a-110); eauto; split; done).
-    iFrame. iNext. iIntros "(HPC & _ & Hr_stk & Ha128)"; iSimpl.
-    iApply wp_pure_step_later;auto;iNext. 
-    iDestruct "Hf2" as "[Hi Hf2]".
-    iApply (wp_bind (fill [SeqCtx])).
-    iApply (wp_move_success_reg _ _ _ _ _ (a-20) (a-21) _ r_t0 _ r_stk
-              with "[HPC Hi Hrt0 Hr_stk]"); eauto; try addr_succ;
-      first apply move_r_i; first apply PermFlows_refl;
-      first (apply isCorrectPC_bounds with (a-0) (a-110); eauto; split; done).
-    iFrame. iNext. iIntros "(HPC & _ & Hrt0 & Hr_stk)"; iSimpl.
-    iApply wp_pure_step_later;auto;iNext.
-    iDestruct "Hf2" as "[Hi Hf2]".
-    iApply (wp_bind (fill [SeqCtx])).
-    iApply (wp_lea_success_z _ _ _ _ _ (a-21) (a-22) _ r_t0 RWLX _ _ _ (a-128) (-7)%Z (a-121)
-              with "[$Hi $Hrt0 $HPC]"); eauto; try addr_succ;
-      first apply lea_z_i;first apply PermFlows_refl;
-      first (apply isCorrectPC_bounds with (a-0) (a-110); eauto; split; done).
-    iNext. iIntros "(HPC & _ & Hrt0)"; iSimpl.
-    iApply wp_pure_step_later;auto;iNext.
-    iDestruct "Hf2" as "[Hi Hf2]".
-    iApply (wp_bind (fill [SeqCtx])).
-    iApply (wp_restrict_success_z _ _ _ _ _ (a-22) (a-23) _ r_t0 RWLX Local (a-120) (a-150) (a-121)
-        local_e with "[Hi HPC Hrt0]"); eauto; try addr_succ;
-      [apply restrict_r_z|apply PermFlows_refl| | | |];
-      first (apply isCorrectPC_bounds with (a-0) (a-110); eauto; split; done).
-    { rewrite epp_local_e /=. auto. }
-    iFrame. iNext. iIntros "(HPC & _ & Hrt0)"; iSimpl.
-    iApply wp_pure_step_later;auto;iNext.
-    iDestruct "Hf2" as "[Hi Hf2]".
-    iApply (wp_bind (fill [SeqCtx])).
-    iApply (wp_GetA_success _ r_t1 _ _ _ _ _ (a-23) _ _ _ (a-24)
-              with "[Hi HPC Hr_t1 Hr_stk]"); eauto;try addr_succ;
-      first apply geta_i; first apply PermFlows_refl;
-      first (apply isCorrectPC_bounds with (a-0) (a-110); eauto; split; done).
-    { iFrame. iFrame. }
-    destruct (reg_eq_dec PC r_stk) as [Hcontr | _]; [inversion Hcontr|].
-    destruct (reg_eq_dec r_stk r_t1) as [Hcontr | _]; [inversion Hcontr|].
-    iNext. iIntros "(HPC & _ & Hr_stk & Hr_t1)"; iSimpl.
-    iApply wp_pure_step_later;auto;iNext.
-    iDestruct "Hf2" as "[Hi Hf2]".
-    iApply (wp_bind (fill [SeqCtx])).
-    iApply (wp_add_sub_lt_success _ r_t1 _ _ _ _ (a-24) _ (inl (z_of (a-128))) _ (inl 1%Z)
-           with "[Hi HPC Hr_t1]"); try addr_succ; eauto; 
-      first (left;apply add_r_z_i); first apply PermFlows_refl;
-      first (apply isCorrectPC_bounds with (a-0) (a-110); eauto; split; done).
-    iFrame. iSplit;[eauto|done]. iNext.
-    destruct (reg_eq_dec r_t1 PC) as [Hcontr | _]; [inversion Hcontr|].
-    destruct (reg_eq_dec r_t1 r_t1); last contradiction.
-    rewrite add_r_z_i. assert (((a-24) + 1)%a = Some (a-25)) as ->;[addr_succ|]. 
-    iIntros "(HPC & _ & _ & _ & Hr_t1)";iSimpl.
-    iApply wp_pure_step_later;auto;iNext.
-    iDestruct "Hf2" as "[Hi Hf2]".
-    iApply (wp_bind (fill [SeqCtx])).
-    iApply (wp_GetE_success _ r_t2 _ _ _ _ _ (a-25) _ _ _ (a-26)
-              with "[Hi HPC Hrt2 Hr_stk]"); eauto;try addr_succ;
-      first apply gete_i; first apply PermFlows_refl;
-      first (apply isCorrectPC_bounds with (a-0) (a-110); eauto; split; done).
-    iFrame. iFrame. iNext.
-    destruct (reg_eq_dec PC r_stk) as [Hcontr | _];[inversion Hcontr|].
-    destruct (reg_eq_dec r_stk r_t2) as [Hcontr | _];[inversion Hcontr|].
-    iIntros "(HPC & _ & Hr_stk & Hr_t2)"; iSimpl.
-    iApply wp_pure_step_later;auto;iNext.
-    iDestruct "Hf2" as "[Hi Hf2]".
-    iApply (wp_bind (fill [SeqCtx])).
-    iApply (wp_subseg_success _ _ _ _ _ (a-26) _ r_stk r_t1 r_t2
-                              RWLX Local (a-120) (a-150) (a-128) 129 150 (a-129) (a-150)
-              with "[Hi HPC Hr_stk Hr_t1 Hr_t2]");eauto;
-      first apply subseg_r_r_i; first apply PermFlows_refl;
-      first (apply isCorrectPC_bounds with (a-0) (a-110); eauto; split; done).
-    { assert (110 ≤ MemNum)%Z; [done|].
-      assert (100 ≤ MemNum)%Z; [done|].
-      rewrite /z_to_addr.
-      destruct ( Z_le_dec 109%Z MemNum),(Z_le_dec 100%Z MemNum); try contradiction.
-      split;[rewrite /(a-109)|rewrite /(a-100)];
-        do 2 f_equal; apply eq_proofs_unicity; decide equality. 
-    }
-    iFrame.
-    assert ((a- 26 + 1)%a = Some (a-27)) as ->;[addr_succ|]. 
-    iNext. iIntros "(HPC & _ & Hr_t1 & Hr_t2 & Hr_stk)"; iSimpl.
-    iApply wp_pure_step_later; auto;iNext. 
-    (* mclear r_stk *)
-    assert (list.last (region_addrs_aux (a-27) 22) = Some (a-48)).
-    { cbn. cbv. do 2 f_equal. apply eq_proofs_unicity. decide equality. }
-    get_genpur_reg "Hr_gen" wsr "[Hrt3 Hr_gen]".
-    get_genpur_reg "Hr_gen" wsr "[Hrt4 Hr_gen]".
-    get_genpur_reg "Hr_gen" wsr "[Hrt5 Hr_gen]".
-    get_genpur_reg "Hr_gen" wsr "[Hrt6 Hr_gen]".
-    iDestruct "Hf2" as "[Hi Hf2]".
-    iApply (mclear_spec (region_addrs_aux (a-27) 22) r_stk (a-48) (a-27) (a-33) (a-43)
-                        pc_p _ pc_g pc_b pc_e RWLX _ Local (a-129) (a-150) (a-128) (a-151) (a-49) 
-              with "[-Hstack]"); try apply PermFlows_refl;
-      try addr_succ; try assumption;[|auto|auto| | | |].  
-    { intros j ai aj Hai Haj.
-      apply (region_addrs_aux_contiguous (a-27) 22 j ai aj); auto.
-      done. }
-    { split; [cbn; f_equal; by apply addr_unique|].
-      split; [addr_succ|cbn; f_equal; by apply addr_unique].  
-    }
-    { apply isCorrectPC_bounds with (a-0) (a-110); eauto; split; done. }
-    { apply isCorrectPC_bounds with (a-0) (a-110); eauto; split; done. }
-    iFrame.
-    iSplitL "Hrt4"; [iNext;iExists _;iFrame|].
-    iSplitL "Hr_t1"; [iNext;iExists _;iFrame|].
-    iSplitL "Hr_t2"; [iNext;iExists _;iFrame|].
-    iSplitL "Hrt3"; [iNext;iExists _;iFrame|].
-    iSplitL "Hrt5"; [iNext;iExists _;iFrame|].
-    iSplitL "Hrt6"; [iNext;iExists _;iFrame|].
-    iSplitL "Hstack_adv"; [iNext;iExists _;iFrame|]. 
-    iNext. iIntros "(HPC & Hr_t1 & Hr_t2 & Hr_t3 & Hr_t4 & Hr_t5 & Hr_t6
-                   & Hr_stk & Hstack_adv & _)".
-    iDestruct "Hf2" as "[Hi Hf2]".
-    clear H3 Hlength'.
-    assert (list.last (region_addrs_aux (a-49) 29) = Some (a-77)).
-    { cbn. cbv. do 2 f_equal. apply eq_proofs_unicity. decide equality. }
-    iApply (rclear_spec (region_addrs_aux (a-49) 29)
-                        (list_difference all_registers [PC; r_stk; r_t0; r_t30])
-                        _ _ _ _ _ (a-49) (a-77) (a-78) with "[-]");
-      try addr_succ; try assumption; try apply PermFlows_refl; auto. 
-    { intros j ai aj Hai Haj.
-      apply (region_addrs_aux_contiguous (a-49) 29 j ai aj); eauto.
-      done. }
-    { apply not_elem_of_list, elem_of_list_here. }
-    { split; (apply isCorrectPC_bounds with (a-0) (a-110); eauto; split; done). }
-    iSplitL "Hr_t1 Hr_t2 Hr_t3 Hr_t4 Hr_t5 Hr_t6 Hr_gen". 
-    { iNext. iExists ((repeat (inl 0%Z) 6) ++ wsr); iSimpl. iFrame. }
-    iSplitL "HPC";[iFrame|].
-    iSplitL "Hi";[iExact "Hi"|].
-    iNext. iIntros "(HPC & Hr_gen & _)".*)
+    (* jmp r_t30 *)
     iPrologue "Hf2".
     iApply (wp_jmp_success _ _ _ _ _ (a-78) with "[Hi HPC Hr1]");
       first apply jmp_i;first apply PermFlows_refl;
       first (apply isCorrectPC_bounds with (a-0) (a-110); eauto; split; done). 
     iFrame. iEpilogue "(HPC & _ & Hr1)"; iSimpl in "HPC".
-    
-
-
-
-    
     (* We have now arrived at the interesting part of the proof: namely the unknown 
        adversary code. In order to reason about unknown code, we must apply the 
        fundamental theorem. To this purpose, we must first define the stsf that will 
@@ -434,8 +288,7 @@ Section lse.
                r_t13; r_t14; r_t15; r_t16; r_t17; r_t18; r_t19; r_t20; r_t21; r_t22; r_t23; r_t24;
                r_t25; r_t26; r_t27; r_t28; r_t29]) as ->; first auto. 
       rewrite /create_gmap_default. iSimpl in "Hr_gen". 
-      repeat (iDestruct "Hr_gen" as "[Hr Hr_gen]";
-              iApply (big_sepM_insert_2 with "[Hr]"); first iFrame).
+      repeat (iDestruct "Hr_gen" as "[Hr Hr_gen]"; iApply (big_sepM_insert_2 with "[Hr]"); first iFrame).
       done. 
     }
     (* r contrains all registers *)
@@ -486,9 +339,14 @@ Section lse.
                        ∗ a- 125 ↦ₐ[RWLX] inl w_4b
                        ∗ a- 126 ↦ₐ[RWLX] inl w_4c
                        ∗ a- 127 ↦ₐ[RWLX] inr (pc_p, pc_g, pc_b, pc_e, a- 78)
-                       ∗ a- 128 ↦ₐ[RWLX] inr (RWLX, Local, a- 120, a- 150, a- 128))%I with "[-Hφ Hs Hstack_adv Hvalid Hmaps Hna Hflag Hr]")
+                                ∗ a- 128 ↦ₐ[RWLX] inr (RWLX, Local, a- 120, a- 150, a- 128))%I
+            with "[-Hφ Hs Hstack_adv Hvalid Hmaps Hna Hflag Hr]")
       as "#Hlocal".
-    { iNext. iFrame. admit. }
+    { iNext. iFrame. rewrite /region_mapsto. 
+      assert (region_addrs (a-121) (a-128) = [a-121; a-122; a-123; a-124; a-125; a-126; a-127; a-128]) as ->.
+      { rewrite /region_addrs. simpl. repeat f_equal; (apply eq_proofs_unicity; decide equality). }
+      repeat (iDestruct "Hstack_own" as "(Ha & Hstack_own)"; iFrame "Ha"). 
+    }
     iAssert (|={⊤}=> ([∗ list] a0 ∈ region_addrs (a-129) (a-150),
                      read_write_cond a0 RWLX (fixpoint interp1)) ∗ region _ ∗ sts_full_world sts_std _)%I
                                            with "[Hstack_adv Hr Hs]" as ">(#Hstack_adv & Hr & Hs)". 
@@ -507,29 +365,31 @@ Section lse.
       - iIntros "%". contradiction.
       - (* invariant for the stack of the adversary *)
         assert (r !! r_stk = Some (inr (RWLX, Local, a-129, a-150, a-128))) as Hr_stk; auto. 
-        rewrite /RegLocate Hr_stk fixpoint_interp1_eq. iSimpl. 
-        iIntros (_). iExists _,_,_,_. (iSplitR; [eauto|]).
-        iExists RWLX. iSplitR; [auto|]. iFrame "#". 
+        rewrite /RegLocate Hr_stk fixpoint_interp1_eq. (* iSimpl.  *)
+        iIntros (_). (* iAlways. iExists _,_,_,_. (iSplitR; [eauto|]). *)
+        iExists RWLX. iSplitR; [auto|].
+        iSplitL.
+        { admit. }
         iAlways.
         rewrite /exec_cond.
         iIntros (a0 r' W' Ha0 HWW'). iNext.
         iApply fundamental.
         + iRight. iRight. done.
-        + iExists RWLX. iSplit; auto. 
+        + iExists RWLX. iSplit; auto. admit.
       - (* continuation *)
         iIntros (_). 
         assert (r !! r_t0 = Some (inr (E, Local, a-120, a-150, a-121))) as Hr_t0; auto. 
         rewrite /RegLocate Hr_t0 fixpoint_interp1_eq. iSimpl. 
         (* prove continuation *)
-        iExists _,_,_,_. iSplit;[eauto|].
+        (* iExists _,_,_,_. iSplit;[eauto|]. *)
         iAlways.
         rewrite /enter_cond. 
         iIntros (r' W' HWW').
         destruct W as [fs' fr' ].
         iNext. iSimpl. 
-        iExists _,_. do 2 (iSplit; [eauto|]).
+        (* iExists _,_.  do 2 (iSplit; [eauto|]).*)
         iIntros "(#[Hfull' Hreg'] & Hmreg' & Hr & Hs & Hna)". 
-        iExists _,_,_,_,_. iSplit; [eauto|rewrite /interp_conf].
+        iSplit; [eauto|rewrite /interp_conf].
         (* get the PC, currently pointing to the activation record *)
         iDestruct (big_sepM_delete _ _ PC with "Hmreg'") as "[HPC Hmreg']".
         { rewrite lookup_insert; eauto. }
