theories/examples/scall.v
@@ -10,6 +10,109 @@ Section scall.
 
   (* Macro for stack calling. Note that the prologue and epilogue does 
      not include storing and loading private state on the stack. *)
+
+  (* helper lemma for the length of the registers *)
+  Ltac iRegNotEq Hne :=
+    repeat (apply not_elem_of_cons in Hne;
+            (let Hneq := fresh "Hneq" in destruct Hne as [Hneq Hne])); auto. 
+
+  Ltac iNotElemOfList :=
+    repeat (apply not_elem_of_cons; split;[auto|]); apply not_elem_of_nil.  
+    
+  Lemma gen_pur_reg_length r1 :
+    r1 ∉ [PC;r_stk] →
+    strings.length (list_difference all_registers [PC; r_stk; r1]) = RegNum - 1.
+  Proof.
+    intros Hne.
+    assert (r1 ∈ all_registers) as Hr1;[apply all_registers_correct|].
+    assert ([PC; r_stk; r1] = [PC; r_stk] ++ [r1]) as Heq; first done. 
+    rewrite Heq. 
+    rewrite list_difference_app.
+    assert (r1 ∈ (list_difference all_registers [PC; r_stk])).
+    { simpl.
+      rewrite /all_registers in Hr1. 
+      (* apply elem_of_cons in Hr1 as [Hcontr | Hr1]. *)
+      assert
+        ([r_t0;r_t1; r_t2; r_t3; r_t4; r_t5; r_t6; r_t7; r_t8; r_t9; r_t10; r_t11;
+          r_t12; r_t13; r_t14; r_t15; r_t16; r_t17; r_t18; r_t19; r_t20; r_t21; r_t22;
+          r_t23; r_t24; r_t25; r_t26; r_t27; r_t28; r_t29; r_t30; r_t31; PC] =
+         [r_t0; r_t1; r_t2; r_t3; r_t4; r_t5; r_t6; r_t7; r_t8; r_t9; r_t10; r_t11;
+          r_t12; r_t13; r_t14; r_t15; r_t16; r_t17; r_t18; r_t19; r_t20; r_t21; r_t22;
+          r_t23; r_t24; r_t25; r_t26; r_t27; r_t28; r_t29; r_t30] ++ [r_t31; PC]) as Hreq; auto. 
+      rewrite Hreq in Hr1. clear Hreq.
+      iRegNotEq Hne. 
+      apply elem_of_app in Hr1 as [Hr1 | Hcontr]; auto.
+      apply elem_of_cons in Hcontr as [? | Hcontr]; first contradiction.
+      apply elem_of_list_singleton in Hcontr; contradiction. 
+    }
+    rewrite list_difference_length; auto.
+    simpl.
+    repeat (apply NoDup_cons; first discharge_not_or).
+    apply NoDup_nil. 
+  Qed.
+
+   Lemma gen_pur_reg_extract {A : Type} `{EqDecision A} (a : A) (l1 l2 : list A) :
+    a ∉ l2 → a ∉ l1 ->
+    list_difference (a :: l1) l2 =
+    a :: list_difference l1 (a :: l2). 
+   Proof.
+     revert l2. induction l1.
+     - intros l2 Hl2 _. simpl. destruct (decide_rel elem_of a l2); done. 
+     - intros l2 Hl2 Hl1.
+       apply not_elem_of_cons in Hl1 as [Hen Hnin]. 
+       simpl. 
+       destruct (decide_rel elem_of a l2);[done|]. 
+       destruct (decide_rel elem_of a0 l2).
+       + destruct (decide_rel elem_of a0 (a :: l2));[apply elem_of_cons in e0 as [Hcontr | Hcontr]; try done|].
+         ++ rewrite list_difference_skip; auto.
+         ++ apply not_elem_of_cons in n0 as [_ Hcontr]. done. 
+       + destruct (decide_rel elem_of a0 (a :: l2));[apply elem_of_cons in e as [Hcontr | Hcontr]; try done|].
+         rewrite list_difference_skip; auto.
+   Qed. 
+
+   Lemma gen_pur_app r1 :
+    r1 ∉ [PC;r_stk;r_t0;r_t1;r_t2;r_t3;r_t4;r_t5;r_t6] →
+    list_difference all_registers [PC; r_stk; r1] =
+    r_t0 :: r_t1 :: r_t2 :: r_t3 :: r_t4 :: r_t5 :: r_t6 :: (list_difference all_registers [r_t0; r_t1;r_t2;r_t3;r_t4;r_t5;r_t6;PC; r_stk; r1]).
+   Proof.
+    intros Hne.
+    iRegNotEq Hne.
+    assert (r1 ∈ all_registers) as Hr1;[apply all_registers_correct|].
+    repeat (rewrite gen_pur_reg_extract;[|iNotElemOfList|iNotElemOfList];f_equiv).
+    assert ([r_t0; r_t1; r_t2; r_t3; r_t4; r_t5; r_t6; PC; r_stk; r1] = [r_t0; r_t1; r_t2; r_t3; r_t4; r_t5; r_t6] ++ [PC; r_stk; r1]) as Happ;[auto|]. 
+    rewrite Happ. 
+    rewrite list_difference_app. 
+    assert ((list_difference all_registers [r_t0; r_t1; r_t2; r_t3; r_t4; r_t5; r_t6]) =
+            [r_t7; r_t8; r_t9; r_t10; r_t11; r_t12; r_t13; r_t14; r_t15; r_t16; r_t17;
+             r_t18; r_t19; r_t20; r_t21; r_t22; r_t23; r_t24; r_t25; r_t26; r_t27; r_t28;
+             r_t29; r_t30; r_t31;PC]) as ->;[auto|].
+    do 7 (rewrite list_difference_skip;[|iNotElemOfList]). done. 
+   Qed.
+
+   Lemma gen_pur_app' r1 :
+    r1 ∉ [PC;r_stk;r_t0;r_t1;r_t2;r_t3;r_t4;r_t5;r_t6] →
+    list_difference all_registers [PC; r_stk; r_t0; r1] =
+    r_t1 :: r_t2 :: r_t3 :: r_t4 :: r_t5 :: r_t6 :: (list_difference all_registers [r_t1;r_t2;r_t3;r_t4;r_t5;r_t6;PC; r_stk; r_t0; r1]).
+   Proof.
+    intros Hne.
+    iRegNotEq Hne.
+    assert (r1 ∈ all_registers) as Hr1;[apply all_registers_correct|].
+    
+    assert ([PC; r_stk; r_t0; r1] = [PC; r_stk; r_t0] ++ [r1]) as ->;[auto|]. 
+    rewrite list_difference_app. 
+    assert ([r_t1; r_t2; r_t3; r_t4; r_t5; r_t6; PC; r_stk; r_t0; r1] = [r_t1; r_t2; r_t3; r_t4; r_t5; r_t6] ++ [PC; r_stk; r_t0; r1]) as Happ;[auto|]. 
+    assert (list_difference all_registers [PC; r_stk; r_t0] =
+            [r_t1; r_t2; r_t3; r_t4; r_t5; r_t6; r_t7; r_t8; r_t9; r_t10; r_t11; r_t12; r_t13; r_t14; r_t15; r_t16;
+             r_t17; r_t18; r_t19; r_t20; r_t21; r_t22; r_t23; r_t24; r_t25; r_t26; r_t27; r_t28; r_t29; r_t30]) as ->;[auto|]. 
+    repeat (rewrite gen_pur_reg_extract;[|iNotElemOfList|iNotElemOfList];f_equiv).
+    assert (r_t1 :: r_t2 :: r_t3 :: r_t4 :: r_t5 :: r_t6 :: [PC; r_stk; r_t0] ++ [r1] =
+            [r_t1;r_t2;r_t3;r_t4;r_t5;r_t6;PC; r_stk; r_t0] ++ [r1]) as ->;[auto|]. 
+    rewrite (list_difference_app _ _ [r1]).
+    assert (list_difference all_registers [r_t1; r_t2; r_t3; r_t4; r_t5; r_t6; PC; r_stk; r_t0] =
+            [r_t7; r_t8; r_t9; r_t10; r_t11; r_t12; r_t13; r_t14; r_t15; r_t16;
+             r_t17; r_t18; r_t19; r_t20; r_t21; r_t22; r_t23; r_t24; r_t25; r_t26; r_t27; r_t28; r_t29; r_t30]) as ->;[auto|]. 
+    do 6 (rewrite list_difference_skip;[|iNotElemOfList]). done. 
+   Qed. 
   
   (* the prologue pushes the activation code, the old pc and stack points, 
      sets up the return capability and adv stack capability, then jumps to adversary code *)
@@ -43,25 +146,89 @@ Section scall.
     mclear_instrs r_stk 10 2 ++ (* 10 and 2 correspond to the offsets to iter in a contiguous mclear *)
     rclear_instrs (list_difference all_registers [PC;r_stk;r_t0;r1]).
 
+  (* Tactic for destructing a list into elements *)
+  Ltac destruct_list l := 
+    match goal with
+    | H : strings.length l = _ |- _ =>
+      let a := fresh "a" in
+      let l' := fresh "l" in
+      destruct l as [|a l']; [inversion H|];
+      repeat (let a' := fresh "a" in
+              destruct l' as [|a' l'];[by inversion H|]);
+      destruct l'; [|by inversion H]
+    end.
+
+  Ltac iPush_z prog stack Hfirst :=
+    match goal with
+    | Hfirst : _ !! _ = Some ?a_first |- _ => 
+      let a_push := fresh "a_push" in
+      let a_rest := fresh "a_rest" in
+      let a1_last := fresh "a1_last" in
+      let cont := fresh "cont" in
+      let Ha1 := fresh "Ha1" in
+      let Ha2 := fresh "Ha2" in
+      let Happ := fresh "Happ" in
+      let Ha1_last := fresh "Ha1_last" in
+      let Ha2_first := fresh "Ha2_first" in
+      let Hlink := fresh "Hlink" in
+      let push1 := fresh "push1" in
+      let push2 := fresh "push2" in
+      let Ha12 := fresh "Ha12" in
+      let w := fresh "w" in
+      iDestruct (contiguous_program_split with prog) as (a_push a_rest a1_last cont) "(Hpush & Hprog & #Hcont)"; [auto|cbv;auto|..];
+      [rewrite app_length;apply PeanoNat.Nat.lt_lt_add_r;cbv;auto;try lia|];
+      iDestruct "Hcont" as %(Ha1 & Ha2 & Happ & Ha1_last & Ha2_first & Hlink);
+      rewrite Happ in Hfirst;
+      iDestruct (big_sepL2_length with "Hpush") as %Hpushlength;
+      destruct (contiguous_2 a_push) as (push1 & push2 & -> & Ha12); auto;
+      simpl in Hfirst; inversion Hfirst; subst; inversion Ha1_last; subst a1_last; clear Hfirst;
+      iApply (push_z_spec with "[-]");last iFrame "Hpush HPC Hr_stk Ha"; [ |auto| |apply Ha12|apply Hlink|auto|]
+    end. 
+
+  Ltac iContiguous_bounds lo mid hi index Ha :=
+    split; [apply incr_list_ge_middle with _ index lo mid in Ha; auto|
+            apply incr_list_le_middle with _ index mid hi in Ha; auto]. 
+
+  Ltac iContiguous_next Ha index :=
+    rewrite /contiguous in Ha; apply Ha with index;auto.
+
+  Ltac iGet_genpur_reg Hr_gen Hwsr wsr ptr :=
+     let w := fresh "wr" in 
+     destruct wsr as [? | w wsr]; first (by inversion Hwsr);
+     iDestruct Hr_gen as ptr.
+
+  Ltac iPrologue l Hl prog := 
+    destruct l; [inversion Hl|];
+    iDestruct prog as "[Hinstr Hprog]";
+    iApply (wp_bind (fill [SeqCtx])).
+
+  Ltac iEpilogue intro_ptrn instr prog :=
+    iNext; iIntros intro_ptrn; iSimpl;
+    iCombine instr prog as prog;
+    iApply wp_pure_step_later;auto;iNext. 
+  
   Definition scall_prologue (a : list Addr) p epilogue_off r1 :=
     ([∗ list] a_i;w_i ∈ a;(scall_prologue_instrs epilogue_off r1), a_i ↦ₐ[p] w_i)%I.
 
   Lemma scall_prologue_spec
-        (* adress arithmetic *) a_r_adv b_r_adv a_act a_cont a_next
+        (* adress arithmetic *) a_r_adv b_r_adv a_act a_cont
         (* scall parameters *) a a_first a_last p' epilogue_off r1
         (* program counter *) p g b e
         (* stack capability *) b_r e_r a_r
         (* continuation *) φ :
     isCorrectPC (inr ((p,g),b,e,a_first)) → isCorrectPC (inr ((p,g),b,e,a_last)) →
+    withinBounds ((RWLX, Local), b_r, e_r, a_act) = true -> withinBounds ((RWLX, Local), b_r, e_r, b_r_adv) = true →
+    (0%a <= e_r)%Z ∧ (0%a <= b_r)%Z → (* This assumption can be removed once we update addresses to be nats *)
     contiguous a →
     a !! 0 = Some a_first -> list.last a = Some a_last ->
     PermFlows p p' →
+    r1 ∉ [PC;r_stk;r_t0;r_t1;r_t2;r_t3;r_t4;r_t5;r_t6] →
 
     (a_r + 1)%a = Some a_act →
-    (a_r + 8)%a = Some a_r_adv →
-    (a_r + 9)%a = Some b_r_adv →
-    (a_first + (13 + epilogue_off))%a = Some a_cont →
-    (a_last + 1)%a = Some a_next →
+    (a_act + 7)%a = Some a_r_adv →
+    (a_act + 8)%a = Some b_r_adv →
+    (a_first + (12 + epilogue_off))%a = Some a_cont →
+    (a_last + 1)%a = Some a_cont →
 
     (▷ scall_prologue a p' epilogue_off r1
    ∗ ▷ PC ↦ᵣ inr ((p,g),b,e,a_first)
@@ -69,7 +236,7 @@ Section scall.
    ∗ ▷ (∃ wsr, [∗ list] r_i;w_i ∈ list_difference all_registers [PC;r_stk;r1]; wsr, r_i ↦ᵣ w_i)
    ∗ ▷ (∃ ws_own, [[a_act, a_r_adv]]↦ₐ[RWLX][[ws_own]]) (* local stack *)
    ∗ ▷ (∃ ws_adv, [[b_r_adv, e_r]]↦ₐ[RWLX][[ws_adv]]) (* adv stack *)
-   ∗ ▷ (PC ↦ᵣ inr (p,g,b,e,a_next)
+   ∗ ▷ (PC ↦ᵣ inr (p,g,b,e,a_cont)
             ∗ r_stk ↦ᵣ inr ((RWLX,Local),b_r_adv,e_r,a_r_adv)
             ∗ r_t0 ↦ᵣ inr ((E,Local),b_r,e_r,a_act)
             ∗ ([∗ list] r_i ∈ list_difference all_registers [PC;r_stk;r_t0;r1], r_i ↦ᵣ inl 0%Z)
@@ -80,30 +247,326 @@ Section scall.
                                              inl w_4b;
                                              inl w_4c;
                                              inr (p,g,b,e,a_cont);
-                                             inr (RWLX,Local,b_r,e_r,b_r_adv)] ]] (* local stack *)
+                                             inr (RWLX,Local,b_r,e_r,a_r_adv)] ]] (* local stack *)
             ∗ [[ b_r_adv, e_r ]] ↦ₐ[RWLX] [[ region_addrs_zeroes b_r_adv e_r ]] (* cleared adv stack *)
             ∗ scall_prologue a p' epilogue_off r1 -∗ 
             WP Seq (Instr Executable) {{ φ }})
    ⊢ WP Seq (Instr Executable) {{ φ }})%I. 
   Proof.
-    iIntros (Hvpc1 Hvpc2 Ha Hfirst Hlast Hfl Hact Hadva Hadvb Hcont Hnext)
+    iIntros (Hvpc1 Hvpc2 Hwb1 Hwb2 Hnonzero Ha Hfirst Hlast Hfl Hne Hact Hadva Hadvb Hcont Hnext)
             "(>Hscall & >HPC & >Hr_stk & >Hr1 & >Hgen_reg & >Hstack & Hφ)".
+    assert (withinBounds ((RWLX, Local), b_r, e_r, a_r_adv) = true) as Hwb3.
+    { apply andb_true_iff.
+      apply andb_true_iff in Hwb2 as [Hba Hae]. apply andb_true_iff in Hwb1 as [Hbact Hacte].
+      revert Hae Hba Hbact Hacte; repeat rewrite Z.leb_le; intros Hae Hba Hbact Hacte.
+      assert (a_r_adv ≤ b_r_adv)%Z as Hle;[apply incr_addr_le with a_act 7 8;auto;lia|]. 
+      assert (a_act ≤ a_r_adv)%Z as Hle';[apply next_le_i with 7;auto;lia|]. lia.
+    }
+    iDestruct "Hgen_reg" as (ws_own) "Hgen_reg".
     rewrite /scall_prologue.
+    (* prepare the local stack for storing the activation record, old PC and old SP *)
+    assert (∃ a1 a2 a3 a4 a5 a6 a7 a8, [a1;a2;a3;a4;a5;a6;a7;a8] = region_addrs a_act a_r_adv)
+      as (a1 & a2 & a3 & a4 & a5 & a6 & a7 & a8 & Hstack_eq).
+    {
+      apply (incr_addr_region_size_iff a_act _ 7) in Hadva as [Hle Hsize].
+      assert (length (region_addrs a_act a_r_adv) = 8) as Hlen;
+        [simpl in Hsize;rewrite -Hsize; apply region_addrs_length;auto|].
+      rewrite /region_mapsto.
+      destruct_list (region_addrs a_act a_r_adv).
+      exists a0,a1,a2,a3,a4,a5,a6,a7. done. 
+    }
+    assert (contiguous (region_addrs a_act a_r_adv)) as Hcontiguous;[apply region_addrs_contiguous|].
+    rewrite -Hstack_eq in Hcontiguous. 
+    rewrite /region_mapsto -Hstack_eq.
+    (* The following length assumptions will let us destruct the stack/program *)
     iDestruct (big_sepL2_length with "Hscall") as %Hlength.
-    iDestruct (contiguous_program_split with "Hscall") as (a1 a2 a1_last a2_first) "(Hpush & Hprog & #Hcont)"; [auto|cbv;auto|..].
-    { rewrite app_length. apply PeanoNat.Nat.lt_lt_add_r. cbv. auto. } (* Make tactic for lengths *)
-    iDestruct "Hcont" as %(Ha1 & Ha2 & Happ & Ha1_last & Ha2_first). 
-    
-    
-    
-  Admitted.
-
-
-
-  Definition scall_epilogue_instrs :=
-    (* pop the restore code *)
-    (* to shorten the program we will do it all at once *)
-    [sub_z_z r_t1 0 7; lea_r r_stk r_t1]. 
+    iDestruct (big_sepL2_length with "Hgen_reg") as %Hlength'. 
+    (* We assert that the first and last elements of the stack are a_acr and a_r_adv *)
+    assert (list.last (region_addrs a_act a_r_adv) = Some a_r_adv) as Hlast_stack.
+    { apply region_addrs_last. apply next_le_i with 7; [lia|auto]. }
+    assert ((region_addrs a_act a_r_adv) !! 0 = Some a_act) as Hfirst_stack.
+    { apply region_addrs_first. apply next_le_i with 7;[lia|auto]. }
+    rewrite -Hstack_eq /= in Hlast_stack. rewrite -Hstack_eq /= in Hfirst_stack.
+    inversion Hlast_stack; inversion Hfirst_stack; subst. clear Hlast_stack Hfirst_stack.
+    (* PUSH ACTIVATION RECORD *)
+    (* push w_1 *)
+    destruct ws_own as [|w ws_own];[inversion Hlength'|]; iDestruct "Hgen_reg" as "[Ha Hstack_own]". 
+    iPush_z "Hscall" "Hgen_reg" Hfirst;[|apply Hwb1|]. 
+    { split; auto. apply isCorrectPC_bounds_alt with a_first a_last; auto.
+      iContiguous_bounds a_first push2 a_last 1 Ha. }
+    iNext. iIntros "(HPC & Hpush & Hr_stk & Ha)".
+    iRename "Hpush" into "Hi". iRename "Ha" into "Hw1". 
+    (* push w_2 *)
+    clear Ha1_last Hlink Hpushlength Ha12 Ha1. rename Ha2_first into Hfirst'.
+    destruct ws_own as [|w1 ws_own];[inversion Hlength'|]; iDestruct "Hstack_own" as "[Ha Hstack_own]". 
+    iPush_z "Hprog" "Hstack_own" Hfirst';[| |iContiguous_next Hcontiguous 0|].
+    { split; apply isCorrectPC_bounds_alt with a_first a_last; auto;
+        [iContiguous_bounds a_first cont a_last 2 Ha|
+         iContiguous_bounds a_first push0 a_last 3 Ha]. }
+    { apply isWithinBounds_bounds_alt with a_act a_r_adv; auto.
+      iContiguous_bounds a_act a2 a_r_adv 1 Hcontiguous. }
+    iNext. iIntros "(HPC & Hpush & Hr_stk & Ha)".
+    iCombine "Hpush" "Hi" as "Hi". iCombine "Ha" "Hw1" as "Hact_frame". 
+    (* push w_3 *)
+    clear Ha1_last Hlink Hpushlength Ha12 Ha1. rename Ha2_first into Hfirst'.
+    destruct ws_own as [|w2 ws_own];[inversion Hlength'|]; iDestruct "Hstack_own" as "[Ha Hstack_own]". 
+    iPush_z "Hprog" "Hstack_own" Hfirst';[| |iContiguous_next Hcontiguous 1|].
+    { split; apply isCorrectPC_bounds_alt with a_first a_last; auto;
+        [iContiguous_bounds a_first cont0 a_last 4 Ha|
+         iContiguous_bounds a_first push3 a_last 5 Ha]. }
+    { apply isWithinBounds_bounds_alt with a_act a_r_adv; auto.
+      iContiguous_bounds a_act a3 a_r_adv 2 Hcontiguous. }
+    iNext. iIntros "(HPC & Hpush & Hr_stk & Ha)".
+    iCombine "Hpush" "Hi" as "Hi". iCombine "Ha" "Hact_frame" as "Hact_frame". 
+    (* push w_4a *)
+    clear Ha1_last Hlink Hpushlength Ha12 Ha1. rename Ha2_first into Hfirst'.
+    destruct ws_own as [|w3 ws_own];[inversion Hlength'|]; iDestruct "Hstack_own" as "[Ha Hstack_own]". 
+    iPush_z "Hprog" "Hstack_own" Hfirst';[| |iContiguous_next Hcontiguous 2|].
+    { split; apply isCorrectPC_bounds_alt with a_first a_last; auto;
+        [iContiguous_bounds a_first cont1 a_last 6 Ha|
+         iContiguous_bounds a_first push4 a_last 7 Ha]. }
+    { apply isWithinBounds_bounds_alt with a_act a_r_adv; auto.
+      iContiguous_bounds a_act a4 a_r_adv 3 Hcontiguous. }
+    iNext. iIntros "(HPC & Hpush & Hr_stk & Ha)".
+    iCombine "Hpush" "Hi" as "Hi". iCombine "Ha" "Hact_frame" as "Hact_frame". 
+    (* push w_4b *)
+    clear Ha1_last Hlink Hpushlength Ha12 Ha1. rename Ha2_first into Hfirst'.
+    destruct ws_own as [|w4 ws_own];[inversion Hlength'|]; iDestruct "Hstack_own" as "[Ha Hstack_own]". 
+    iPush_z "Hprog" "Hstack_own" Hfirst';[| |iContiguous_next Hcontiguous 3|].
+    { split; apply isCorrectPC_bounds_alt with a_first a_last; auto;
+        [iContiguous_bounds a_first cont2 a_last 8 Ha|
+         iContiguous_bounds a_first push5 a_last 9 Ha]. }
+    { apply isWithinBounds_bounds_alt with a_act a_r_adv; auto.
+      iContiguous_bounds a_act a5 a_r_adv 4 Hcontiguous. }
+    iNext. iIntros "(HPC & Hpush & Hr_stk & Ha)".
+    iCombine "Hpush" "Hi" as "Hi". iCombine "Ha" "Hact_frame" as "Hact_frame". 
+    (* push w_4a *)
+    clear Ha1_last Hlink Hpushlength Ha12 Ha1. rename Ha2_first into Hfirst'.
+    destruct ws_own as [|w5 ws_own];[inversion Hlength'|]; iDestruct "Hstack_own" as "[Ha Hstack_own]".
+    iPush_z "Hprog" "Hstack_own" Hfirst';[| |iContiguous_next Hcontiguous 4|].
+    { split; apply isCorrectPC_bounds_alt with a_first a_last; auto;
+        [iContiguous_bounds a_first cont3 a_last 10 Ha|
+         iContiguous_bounds a_first push6 a_last 11 Ha]. }
+    { apply isWithinBounds_bounds_alt with a_act a_r_adv; auto.
+      iContiguous_bounds a_act a6 a_r_adv 5 Hcontiguous. }
+    iNext. iIntros "(HPC & Hpush & Hr_stk & Ha)".
+    iCombine "Hpush" "Hi" as "Hi". iCombine "Ha" "Hact_frame" as "Hact_frame". 
+    clear Ha5 Ha4 Ha3 Ha0 Ha2 Ha1 Ha6 Hlink Hpushlength Ha1_last.
+    (* PUSH OLD PC *)
+    (* some general purpose registers *)
+    iDestruct "Hr1" as (wsr) "Hr_gen".
+    iDestruct (big_sepL2_length with "Hr_gen") as %Hreglength.
+    rewrite (gen_pur_reg_length r1) /= in Hreglength;[|iRegNotEq Hne;iNotElemOfList].
+    rewrite gen_pur_app;[|auto]. 
+    iGet_genpur_reg "Hr_gen" Hreglength wsr "[Hrt0 Hr_gen]".
+    iGet_genpur_reg "Hr_gen" Hreglength wsr "[Hrt1 Hr_gen]".
+    (* move r_t1 PC *)
+    do 2 (destruct a_rest0; [inversion Hlength|]).
+    inversion Ha2_first as [Heq]. rewrite -Heq. 
+    iDestruct "Hprog" as "[Hinstr Hprog]".
+    iApply (wp_bind (fill [SeqCtx])).
+    iApply (wp_move_success_reg_fromPC with "[$Hinstr $Hrt1 $HPC]");
+      [apply move_r_i|apply Hfl| |iContiguous_next Ha 12|auto|].
+    { apply isCorrectPC_bounds_alt with a_first a_last;auto;iContiguous_bounds a_first a a_last 12 Ha. }
+    iEpilogue "(HPC & Hinstr & Hr_t1)" "Hinstr" "Hi". 
+    (* lea r_t1 epilogue_off *)
+    iPrologue a_rest0 Hlength "Hprog". 
+    (* we first need to make some assertions about the increase of the address a *)
+    assert ((a + epilogue_off)%a = Some a_cont) as Hepilogue.
+    { rewrite -Hcont (addr_add_assoc _ a);[auto|].
+      apply (contiguous_incr_addr _ 12 _ _ Ha); auto. }
+    iApply (wp_lea_success_z with "[$Hinstr $Hr_t1 $HPC]");
+      [apply lea_z_i|apply Hfl| |iContiguous_next Ha 13|apply Hepilogue|auto|..].
+    {  apply isCorrectPC_bounds_alt with a_first a_last;auto;iContiguous_bounds a_first a0 a_last 13 Ha. }
+    { inversion Hvpc1 as [?????? Hpc_p]; 
+        destruct Hpc_p as [Hpc_p | [Hpc_p | Hpc_p] ]; congruence. }
+    iEpilogue "(HPC & Hinstr & Hrt_1)" "Hinstr" "Hi". 
+    (* PUSH R_T1 *)
+    (* lea r_stk 1 *)
+    iPrologue a_rest0 Hlength "Hprog". 
+    iApply (wp_lea_success_z with "[$Hinstr $Hr_stk $HPC]");
+      [apply lea_z_i|apply Hfl| |iContiguous_next Ha 14|iContiguous_next Hcontiguous 5|auto|auto|].
+    { apply isCorrectPC_bounds_alt with a_first a_last;auto;iContiguous_bounds a_first a1 a_last 14 Ha. }
+    iEpilogue "(HPC & Hinstr & Hr_stk)" "Hinstr" "Hi".
+    (* store r_stk r_t1 *)
+    iPrologue a_rest0 Hlength "Hprog".
+    destruct ws_own;[inversion Hlength'|].
+    iDestruct "Hstack_own" as "[Ha7 Hstk_own]". 
+    iApply (wp_store_success_reg with "[$HPC $Hinstr $Hrt_1 $Hr_stk $Ha7]");
+      [apply store_r_i|apply Hfl|apply PermFlows_refl| |iContiguous_next Ha 15|split;auto|by right;left|auto|].
+    { apply isCorrectPC_bounds_alt with a_first a_last;auto;iContiguous_bounds a_first a8 a_last 15 Ha. }
+    { apply isWithinBounds_bounds_alt with a_act a_r_adv; auto.
+      iContiguous_bounds a_act a7 a_r_adv 6 Hcontiguous. }  
+    iEpilogue "(HPC & Hinstr & Hr_t1 & Hr_stk & Ha7)" "Hinstr" "Hi".
+    iCombine "Ha7" "Hact_frame" as "Hact_frame".
+    (* STORE OLD SP *)
+    (* lea r_stk 1 *)
+    iPrologue a_rest0 Hlength "Hprog". 
+    iApply (wp_lea_success_z with "[$Hinstr $Hr_stk $HPC]");
+      [apply lea_z_i|apply Hfl| |iContiguous_next Ha 16|iContiguous_next Hcontiguous 6|auto|auto|].
+    { apply isCorrectPC_bounds_alt with a_first a_last;auto;iContiguous_bounds a_first a9 a_last 16 Ha. }
+    iEpilogue "(HPC & Hinstr & Hr_stk)" "Hinstr" "Hi".
+    (* store r_stk r_stk *)
+    iPrologue a_rest0 Hlength "Hprog".
+    destruct ws_own;[inversion Hlength'|].
+    iDestruct "Hstk_own" as "[Ha8 Hstk_own]". 
+    iApply (wp_store_success_reg_same with "[$HPC $Hinstr $Hr_stk $Ha8]");
+      [apply store_r_i|apply Hfl|apply PermFlows_refl| |iContiguous_next Ha 17|split;auto|by right;left|auto|]. 
+    { apply isCorrectPC_bounds_alt with a_first a_last;auto;iContiguous_bounds a_first a10 a_last 17 Ha. }
+    iEpilogue "(HPC & Hinstr & Hr_stk & Ha_r_adv)" "Hinstr" "Hi".
+    iCombine "Ha_r_adv" "Hact_frame" as "Hact_frame".
+    (* PREPARE RETURN CAP *)
+    (* move r_t0 r_stk *)
+    iPrologue a_rest0 Hlength "Hprog". 
+    iApply (wp_move_success_reg with "[$HPC $Hinstr $Hrt0 $Hr_stk]");
+      [apply move_r_i|apply Hfl| |iContiguous_next Ha 18|auto|]. 
+    { apply isCorrectPC_bounds_alt with a_first a_last;auto;iContiguous_bounds a_first a11 a_last 18 Ha. }
+    iEpilogue "(HPC & Hinstr & Hr_t0 & Hr_stk)" "Hinstr" "Hi".
+    (* lea r_t0 -7 *)
+    (* assert that the activation frame starts at a_act *)
+    assert ((a_r_adv + -7)%a = Some a_act) as Ha_act.
+    { rewrite -(addr_add_assoc a_act _ 7);auto. assert ((7 + -7) = 0)%Z as ->;[lia|]. apply addr_add_0. }
+    iPrologue a_rest0 Hlength "Hprog".
+    iApply (wp_lea_success_z with "[$HPC $Hinstr $Hr_t0]");
+      [apply lea_z_i|apply Hfl| |iContiguous_next Ha 19|apply Ha_act|auto..]. 
+    { apply isCorrectPC_bounds_alt with a_first a_last;auto;iContiguous_bounds a_first a12 a_last 19 Ha. }
+    iEpilogue "(HPC & Hinstr & Hr_t0)" "Hinstr" "Hi". 
+    (* restrict r_t0 (Local,E) *)
+    iPrologue a_rest0 Hlength "Hprog". 
+    iApply (wp_restrict_success_z with "[$HPC $Hinstr $Hr_t0]");
+      [apply restrict_r_z|apply Hfl| |iContiguous_next Ha 20|rewrite epp_local_e;auto|auto|].
+    { apply isCorrectPC_bounds_alt with a_first a_last;auto;iContiguous_bounds a_first a13 a_last 20 Ha. }
+    iEpilogue "(HPC & Hinstr & Hr_t0)" "Hinstr" "Hi".
+    (* RESTRICT STACK CAP *)
+    (* geta r_t1 r_stk *)
+    iPrologue a_rest0 Hlength "Hprog". 
+    iApply (wp_GetA_success with "[$HPC $Hinstr Hr_t1 Hr_stk]");
+      [apply geta_i|apply Hfl| |iContiguous_next Ha 21|auto|simpl;iFrame|iSimpl]. 
+    { apply isCorrectPC_bounds_alt with a_first a_last;auto;iContiguous_bounds a_first a14 a_last 21 Ha. }
+    iEpilogue "(HPC & Hinstr & Hr_stk & Hr_t1)" "Hinstr" "Hi". 
+    (* add r_t1 r_t1 1 *)
+    iPrologue a_rest0 Hlength "Hprog". 
+    iApply (wp_add_sub_lt_success with "[$HPC $Hinstr Hr_t1]");
+      [left;apply add_r_z_i|apply Hfl| |iSimpl;iFrame;eauto|iSimpl;rewrite add_r_z_i]. 
+    { apply isCorrectPC_bounds_alt with a_first a_last;auto;iContiguous_bounds a_first a15 a_last 22 Ha. }
+    assert ((a15 + 1)%a = Some a16) as ->;[iContiguous_next Ha 22|]. 
+    iEpilogue "(HPC & Hinstr & _ & _ & Hr_t1)" "Hinstr" "Hi". 
+    (* gete r_t2 r_stk *)
+    iGet_genpur_reg "Hr_gen" Hreglength wsr "[Hr_t2 Hr_gen]".
+    iPrologue a_rest0 Hlength "Hprog". 
+    iApply (wp_GetE_success with "[$HPC $Hinstr Hr_t2 Hr_stk]");
+      [apply gete_i|apply Hfl| |iContiguous_next Ha 23|auto|iSimpl;iFrame|iSimpl]. 
+    { apply isCorrectPC_bounds_alt with a_first a_last;auto;iContiguous_bounds a_first a16 a_last 23 Ha. }
+    iEpilogue "(HPC & Hinstr & Hr_stk & Hr_t2)" "Hinstr" "Hi". 
+    (* subseg r_stk r_t1 r_t2 *)
+    assert (z_to_addr (a_r_adv + 1) = Some b_r_adv) as Hb_r_adv.
+    { assert ((a_r_adv + 1)%a = Some b_r_adv) as temp;[rewrite -(addr_add_assoc a_act _ 7);auto|auto]. }
+    assert (z_to_addr e_r = Some e_r) as He_r.
+    { rewrite /z_to_addr. destruct (Z_le_dec e_r MemNum);destruct e_r;[f_equiv;by apply z_of_eq|].
+      exfalso. clear Hwb1 Hwb2 Hwb3 Hnonzero. simpl in n. revert fin. rewrite Z.leb_le. done. }
+    iPrologue a_rest0 Hlength "Hprog". 
+    iApply (wp_subseg_success with "[$HPC $Hinstr $Hr_stk $Hr_t1 $Hr_t2]");
+      [apply subseg_r_r_i|apply Hfl| |eauto|auto|auto|..].
+    { apply isCorrectPC_bounds_alt with a_first a_last;auto;iContiguous_bounds a_first a17 a_last 24 Ha. }
+    { repeat (apply andb_true_iff;split);destruct Hnonzero as [Hnz1 Hnz2] ;apply Z.leb_le;auto;last lia.
+      apply Store.withinBounds_le_addr in Hwb3 as [Hwb3 _]. 
+      trans a_r_adv; auto.
+      assert ((a_r_adv + 1)%a = Some b_r_adv) as temp;[rewrite -(addr_add_assoc a_act _ 7);auto|].
+      apply next_le_i with 1;[lia|auto]. 
+    } 
+    assert ((a17 + 1)%a = Some a18) as ->;[iContiguous_next Ha 24|].
+    iEpilogue "(HPC & Hinstr & Hr_t1 & Hr_t2 & Hr_stk)" "Hinstr" "Hi".
+    (* MCLEAR *)
+    assert ([a_first; push2] ++ [cont; push0] ++ [cont0; push3] ++ [cont1; push4] ++ [cont2; push5] ++ [cont3; push6]
+                             ++ a :: a0 :: a1 :: a8 :: a9 :: a10 :: a11 :: a12 :: a13 :: a14 :: a15 :: a16 :: a17 :: a18 :: a_rest0 =
+            [a_first; push2; cont; push0; cont0; push3; cont1; push4; cont2; push5; cont3; push6;
+             a; a0; a1; a8; a9; a10; a11; a12; a13; a14; a15; a16; a17]
+              ++ a18 :: a_rest0) as Happeq;[auto|].
+    apply contiguous_app with _ _ a17 a18 _ in Happeq as (Hcont1 & Hcont2 & Hlink); auto. 
+    iDestruct (contiguous_program_split with "Hprog") as (mclear_addrs rclear_addrs mclear_last rclear_first) "(Hmclear & Hrclear & #Hcont)";[auto|simpl;lia| |]. 
+    { rewrite /rclear_instrs map_length helper1;[lia|iRegNotEq Hne|apply all_registers_correct]. }
+    iDestruct "Hcont" as %(Hcont21 & Hcont22 & Happeq' & Hlast1 & Hfirst1 & Hlink').
+    iDestruct (big_sepL2_length with "Hmclear") as %Hmclear_length.
+    assert (7 < (length mclear_addrs)) as Hlt7;[rewrite Hmclear_length /=;lia|].
+    assert (17 < (length mclear_addrs)) as Hlt17;[rewrite Hmclear_length /=;lia|].
+    apply lookup_lt_is_Some_2 in Hlt7 as [ai Hai]. 
+    apply lookup_lt_is_Some_2 in Hlt17 as [aj Haj].
+    assert (([a_first; push2] ++ [cont; push0] ++ [cont0; push3] ++ [cont1; push4] ++ [cont2; push5] ++
+               [cont3; push6] ++ a :: a0 :: a1 :: a8 :: a9 :: a10 :: a11 :: a12 :: a13 :: a14 :: a15 :: a16 :: a17 :: a18 :: a_rest0)
+                !! (25 + (strings.length mclear_addrs - 1)) = Some mclear_last) as Heqapp.
+    { repeat rewrite (cons_middle); repeat rewrite (app_assoc _ _ (a18 :: a_rest0)).
+      rewrite (lookup_app_r _ (a18 :: a_rest0));[|simpl;lia]; rewrite Happeq'.
+      rewrite lookup_app_l /=;
+              [rewrite PeanoNat.Nat.sub_0_r;rewrite -last_lookup; auto|
+               rewrite PeanoNat.Nat.sub_0_r; apply PeanoNat.Nat.sub_lt;[|lia];
+               destruct mclear_addrs; [inversion Hlast1|simpl;lia] ]. }
+    iApply (mclear_spec with "[-]"); last (rewrite /region_mapsto; iFrame "HPC Hr_stk Hstack");
+      [apply Hcont21| |apply Hlast1|auto| | | |
+       apply Hfl|apply PermFlows_refl|apply Hlink'|..]. 
+    { rewrite -(lookup_app_l _ rclear_addrs);[|rewrite Hmclear_length /=;lia]. rewrite -Happeq'. auto. }
+    { split;[eauto|split;[|eauto] ]. apply (contiguous_incr_addr_middle mclear_addrs 7 10 ai aj); auto. }
+    { apply isCorrectPC_bounds_alt with a_first a_last;auto;iContiguous_bounds a_first a18 a_last 25 Ha. }
+    { apply isCorrectPC_bounds_alt with a_first a_last;auto.
+      iContiguous_bounds a_first mclear_last a_last (25 + (length mclear_addrs - 1)) Ha. }
+    { apply andb_true_iff in Hwb2 as [_ Hwb2]. by apply Z.leb_le. }
+    rewrite /mclear.
+    destruct (strings.length mclear_addrs =? strings.length (mclear_instrs r_stk 10 2))%nat eqn:Hcontr;
+      [|rewrite Hmclear_length in Hcontr;inversion Hcontr].
+    iFrame "Hmclear".
+    iGet_genpur_reg "Hr_gen" Hreglength wsr "[Hr_t3 Hr_gen]".
+    iGet_genpur_reg "Hr_gen" Hreglength wsr "[Hr_t4 Hr_gen]".
+    iGet_genpur_reg "Hr_gen" Hreglength wsr "[Hr_t5 Hr_gen]".
+    iGet_genpur_reg "Hr_gen" Hreglength wsr "[Hr_t6 Hr_gen]".
+    iSplitL "Hr_t4". iNext; eauto. 
+    iSplitL "Hr_t1". iNext; eauto. 
+    iSplitL "Hr_t2". iNext; eauto. 
+    iSplitL "Hr_t3". iNext; eauto. 
+    iSplitL "Hr_t5". iNext; eauto. 
+    iSplitL "Hr_t6". iNext; eauto.
+    iNext. iIntros "(HPC & Hr_t1 & Hr_t2 & Hr_t3 & Hr_t4 & Hr_t5 & Hr_t6 & Hr_stk & Hstack_adv & Hmclear)".
+    (* RCLEAR *)
+    iDestruct (big_sepL2_length with "Hrclear") as %Hrclear_length.
+    rewrite map_length helper1 in Hrclear_length;[|iRegNotEq Hne|apply all_registers_correct]. 
+    assert (list.last rclear_addrs = Some a_last) as Hr_last.
+    { rewrite Happeq' in Hlast. simpl in Hlast.
+      rewrite (last_app_iff (a17 :: mclear_addrs)).
+      split;[rewrite Hrclear_length;lia|]. auto. }
+    iApply (rclear_spec with "[-]"); last (iFrame "HPC Hrclear");
+      [auto|apply Hr_last|apply Hnext|apply not_elem_of_list;apply elem_of_cons; by left| | |apply Hfl|..].
+    { destruct rclear_addrs;inversion Hfirst1. done. }
+    { split; auto. apply isCorrectPC_bounds_alt with a_first a_last;auto.
+      split;[|apply incr_list_le with rclear_addrs; auto].
+      trans mclear_last. 
+      - apply incr_list_ge_middle with _ _ a_first _ in Heqapp; auto. 
+      - apply next_le_i with 1; auto; lia. }
+    iSplitL "Hr_t1 Hr_t2 Hr_t3 Hr_t4 Hr_t5 Hr_t6 Hr_gen".
+    { iNext. iApply region_addrs_exists.
+      rewrite gen_pur_app';[|iRegNotEq Hne;iNotElemOfList]. 
+      iSplitL "Hr_t1";[eauto|].
+      iSplitL "Hr_t2";[eauto|].
+      iSplitL "Hr_t3";[eauto|].
+      iSplitL "Hr_t4";[eauto|].
+      iSplitL "Hr_t5";[eauto|].
+      iSplitL "Hr_t6";[eauto|].
+      iApply region_addrs_exists.
+      assert ([r_t1; r_t2; r_t3; r_t4; r_t5; r_t6; PC; r_stk] ++ r_t0 :: [r1] =
+              [r_t1; r_t2; r_t3; r_t4; r_t5; r_t6; PC; r_stk; r_t0; r1]) as Heq';[auto|]. 
+      assert ([r_t1; r_t2; r_t3; r_t4; r_t5; r_t6; PC; r_stk; r_t0; r1] ≡ₚ
+              [r_t0; r_t1; r_t2; r_t3; r_t4; r_t5; r_t6; PC; r_stk; r1]) as Hperm.
+      { rewrite -Heq'. rewrite -Permutation_middle. done. }
+      apply list_difference_Permutation with all_registers _ _ in Hperm. rewrite Hperm.  
+      iExists wsr. iFrame. 
+    }
+    iNext. iIntros "(HPC & Hgen_reg & Hrclear)".
+    iApply "Hφ". rewrite epp_local_e. iFrame "HPC Hr_stk Hr_t0 Hgen_reg Hstack_adv".
+    iSplitL "Hact_frame".
+    - iDestruct "Hact_frame" as "(Ha_r_adv & Ha7 & Ha6 & Ha5 & Ha4 & Ha3 & Ha2 & Ha_act)".
+      iFrame. done.
+    - rewrite Happeq'.
+      iDestruct "Hi" as "(Ha17 & Ha16 & Ha15 & Ha14 & Ha13 & Ha12 & Ha11 & Ha10 & Ha9 &
+                          Ha8 & Ha1 & Ha0 & Ha & Hpush6 & Hpush5 & Hpush4 & Hpush3 & Hpush0 & Hpush2)".
+      iFrame. Unshelve. exact (inl 0%Z).
+  Qed. 
 
 
 End scall. 
